EarleyTest/Basic.lean
@@ -6,41 +6,39 @@ This suite tests the basic functionality around EarleyItems
 
 It tests the general mathlib API and basic usage of the functions for the example Grammar G
   G = ({S, a}, {a}, {S -> aS | a}, S) with L(G) = a⁺
-
-TODO: write Tests for Repr
 -/
 
 /- Simple Usage Examples for Mathlib Types -/
-inductive NT where
-| S : NT
-deriving Repr
+inductive N where
+| S : N
+deriving BEq, Repr
 
 inductive T where
 | a : T
-deriving Repr
+deriving BEq, Repr
 
-def exRule1 : ContextFreeRule T NT where
-  input := NT.S
+def exRule1 : ContextFreeRule T N where
+  input := N.S
   output := [Symbol.terminal T.a]
 
-def exRule2 : ContextFreeRule T NT where
-  input := NT.S
-  output := [Symbol.terminal T.a, Symbol.nonterminal NT.S]
+def exRule2 : ContextFreeRule T N where
+  input := N.S
+  output := [Symbol.terminal T.a, Symbol.nonterminal N.S]
 
 /--
-info: NT.S → [T.a, NT.S]
+info: N.S → [T.a, N.S]
 -/
 #guard_msgs in
 #eval exRule2
 
-def exRules : Finset (ContextFreeRule T NT) where
+def exRules : Finset (ContextFreeRule T N) where
   val := { exRule1, exRule2 }
   nodup := by simp [exRule1, exRule2]
 
--- TODO: understand the design decision to not have NT as a parameter
+-- TODO: understand the design decision to not have N as a parameter
 -- (or atleast implicit from the `initial` field!)
 def G : ContextFreeGrammar T :=
-  { NT := NT, initial := NT.S, rules := exRules }
+  { NT := N, initial := N.S, rules := exRules }
 
 /-
 Example theorems that the grammar can generate a certain word.
@@ -49,17 +47,17 @@ TODO: Im overlooking some good lemmas right? This shouldnt need that much unfold
 Maybe the idea would be some mem_ lemmas?
 Or people dont think this is a noteworthy thing to prove.
 -/
-theorem exProduces : G.Produces [Symbol.nonterminal NT.S] [Symbol.terminal T.a] := by
+theorem exProduces : G.Produces [Symbol.nonterminal N.S] [Symbol.terminal T.a] := by
   unfold G
   unfold ContextFreeGrammar.Produces
   simp [exRules]
   apply Or.inl
   apply ContextFreeRule.Rewrites.head
 
-theorem exGenerates (h : G.Produces [Symbol.nonterminal NT.S] [Symbol.terminal T.a]) : G.Generates [Symbol.terminal T.a] := by
+theorem exGenerates (h : G.Produces [Symbol.nonterminal N.S] [Symbol.terminal T.a]) : G.Generates [Symbol.terminal T.a] := by
   unfold ContextFreeGrammar.Generates
   unfold ContextFreeGrammar.Derives
-  apply @Relation.ReflTransGen.tail (b:= [Symbol.nonterminal NT.S])
+  apply @Relation.ReflTransGen.tail (b:= [Symbol.nonterminal N.S])
   . unfold G
     apply Relation.ReflTransGen.refl
   . exact h
@@ -78,70 +76,115 @@ info: {w | G.Generates (List.map Symbol.terminal w)} : Set (List T)
 
 open Earley.EarleyRecognizer
 
-/--
-info: ([], [T.a, NT.S])
--/
-#guard_msgs in
-#eval splitRuleAt exRule2 0
+theorem split0 :
+    splitRuleAt exRule2 0 = ⟨[], [Symbol.terminal T.a, Symbol.nonterminal N.S]⟩
+  := rfl
+theorem split1 :
+    splitRuleAt exRule2 1 = ⟨[Symbol.terminal T.a], [Symbol.nonterminal N.S]⟩
+  := rfl
+theorem split2 :
+    splitRuleAt exRule2 2 = ⟨[Symbol.terminal T.a, Symbol.nonterminal N.S], []⟩
+  := rfl
+theorem split3 :
+    splitRuleAt exRule2 3 = ⟨[Symbol.terminal T.a, Symbol.nonterminal N.S], []⟩
+  := rfl
 
-/--
-info: ([T.a], [NT.S])
--/
-#guard_msgs in
-#eval splitRuleAt exRule2 1
-
-/--
-info: ([T.a, NT.S], [])
--/
-#guard_msgs in
-#eval splitRuleAt exRule2 2
-
-/--
-info: ([T.a, NT.S], [])
--/
-#guard_msgs in
-#eval splitRuleAt exRule2 3
-
-def exItem1 : EarleyItem T NT where
+def exItem1 : EarleyItem T N where
   rule := exRule2
   position := 0
   startItem := 0
   endItem := 0
 
-def exItem2 : EarleyItem T NT :=
-  { exItem1 with position := 1 }
+def exItem2 : EarleyItem T N :=
+  { exItem1 with position := 1, startItem := 1, endItem := 2 }
 
-def exItem3 : EarleyItem T NT :=
-  { exItem1 with position := 2, startItem := 1 }
+def exItem3 : EarleyItem T N :=
+  { exItem1 with position := 2, startItem := 1 , endItem := 0 }
+
+def exItem4 : EarleyItem T N :=
+  { exItem1 with position := 3, startItem := 1 , endItem := 2 }
+
+def exItem5 : EarleyItem T N where
+  rule := exRule1
+  position := 1
+  startItem := 0
+  endItem := 1
 
 /--
-info: NT.S → [T.a] @ [NT.S] w/ (0, 0)
+info: N.S → [] @ [T.a, N.S] w/ (0, 0)
+-/
+#guard_msgs in
+#eval exItem1
+
+/--
+info: N.S → [T.a] @ [NT.S] w/ (1, 2)
 -/
 #guard_msgs in
 #eval exItem2
 
 /--
-info: some T.a
+info: N.S → [T.a, N.S] @ [] w/ (1, 0)
 -/
 #guard_msgs in
-#eval nextSymbol exItem1
+#eval exItem3
 
 /--
-info: some NT.S
+info: N.S → [T.a, N.S] @ [] w/ (1, 2)
 -/
 #guard_msgs in
-#eval nextSymbol exItem2
+#eval exItem4
 
-/--
-info: none
--/
-#guard_msgs in
-#eval nextSymbol exItem3
+theorem next1 : nextSymbol exItem1 = some (Symbol.terminal T.a) := rfl
+theorem next2 : nextSymbol exItem2 = some (Symbol.nonterminal N.S) := rfl
+theorem next3 : nextSymbol exItem3 = none := rfl
 
-def exW : String := "aaa"
+theorem complete1 : isComplete exItem1 = false := rfl
+theorem complete2 : isComplete exItem2 = false := rfl
+theorem complete3 : isComplete exItem3 = true := rfl
+theorem complete4 : isComplete exItem4 = false := rfl
 
-#check isComplete
+-- TODO: this is already derived, but I want to understand why this isnt enough
+instance : BEq N where
+  beq fst snd := match fst,snd with
+    | N.S, N.S => true
 
-#check isFinished
+-- TODO: I don't understand why
+instance : BEq G.NT where
+  beq fst snd := match fst,snd with
+    | N.S, N.S => true
 
-#check isWellFormed
+def exW1 : String := "a"
+def exW2 : String := "aaa"
+theorem finished1 : isFinished G exItem1 exW1 = false := rfl
+theorem finished2 : isFinished G exItem2 exW1 = false := rfl
+theorem finished3 : isFinished G exItem3 exW1 = false := rfl
+theorem finished4 : isFinished G exItem4 exW1 = false := rfl
+theorem finished5 : isFinished G exItem5 exW1 = true := rfl
+
+-- These just wait for lemmas, which I will require anyway for the proofs right?
+  -- [Finset.mem_toList]
+theorem wf1 : isWellFormed G exItem1 exW1 := by
+  rw [isWellFormed, exItem1]
+  unfold G
+  unfold exRules
+  simp
+  sorry
+
+theorem wf2 : ¬isWellFormed G exItem2 exW1 := by
+  rw [isWellFormed, exItem2, exW1]
+  simp [String.length]
+
+theorem wf3 : ¬isWellFormed G exItem3 exW2 := by
+  rw [isWellFormed, exItem3]
+  simp
+
+theorem wf4 : ¬isWellFormed G exItem4 exW2 := by
+  rw [isWellFormed, exItem4, exItem1, exW2, exRule2]
+  simp [List.length]
+
+theorem wf5 : isWellFormed G exItem5 exW2 := by
+  rw [isWellFormed, exItem5, exW2]
+  unfold G
+  unfold exRules
+  simp [String.length, List.length]
+  sorry
